books/centaur/fgl/satlink-sat.lisp
@@ -34,248 +34,108 @@
 (include-book "pathcond")
 (include-book "interp-st-bfrs-ok")
 (include-book "sat-stub")
-(include-book "centaur/satlink/top" :dir :system)
+(include-book "centaur/aignet/cube-sat" :dir :system)
 (local (std::add-default-post-define-hook :fix))
 (local (include-book "std/lists/resize-list" :dir :system))
 
+(defprod fgl-satlink-monolithic-sat-config
+  ((ignore-pathcond booleanp :default t)
+   (ignore-constraint booleanp :default nil)
+   (satlink-config-override :default nil)
+   (transform booleanp :default nil)
+   (transform-config-override :default nil)))
 
-(local
- (defsection logicman->aignet->ipasir-lemmas
 
-   (defthm cdr-of-nthcdr
-     (equal (cdr (nthcdr n x))
-            (nthcdr n (cdr x))))
-
-   (defthm hons-assoc-equal-in-pairlis-numlist
-     (implies (and (natp start) (natp n))
-              (equal (cdr (hons-assoc-equal n (pairlis$ (numlist start 1 k) (nthcdr start x))))
-                     (and (< (- n start) (nfix k))
-                          (<= start n)
-                          (nth n x))))
-     :hints(("Goal" :in-theory (enable car-of-nthcdr)
-             :induct (numlist start 1 k))))
-
-   (defthm hons-assoc-equal-in-pairlis-numlist-base
-     (implies (natp n)
-              (equal (cdr (hons-assoc-equal n (pairlis$ (numlist 0 1 k) x)))
-                     (and (< n (nfix k))
-                          (nth n x))))
-     :hints(("Goal" :use ((:instance hons-assoc-equal-in-pairlis-numlist
-                           (start 0)))
-             :in-theory (disable hons-assoc-equal-in-pairlis-numlist))))
-
-   (local (include-book "theory"))
-   
-   (defthm nth-alist-to-bitarr-of-pairlis$
-     (acl2::bit-equiv (nth n (alist-to-bitarr k (pairlis$ (acl2::numlist 0 1 k) bits) nil))
-                      (if (< (nfix n) (nfix k))
-                          (bool->bit (nth n bits))
-                        0)))
-   
-   (defthm alist-to-bitarr-of-pairlis$-under-bits-equiv
-     (acl2::bits-equiv (alist-to-bitarr k (pairlis$ (acl2::numlist 0 1 k) bools) nil)
-                       (take k (bools->bits bools)))
-     :hints(("Goal" :in-theory (enable acl2::bits-equiv)
-             :do-not-induct t)))
-   
-   (defthm bools->bits-of-bits->bools-under-bits-equiv
-     (acl2::bits-equiv (bools->bits (bits->bools x)) x)
-     :hints(("Goal" :in-theory (enable acl2::bits-equiv))))
-
-   (defthm eval-lit-of-lit-negate-cond
-     (implies (bitp val)
-              (equal (equal (satlink::eval-lit (satlink::lit-negate-cond lit neg) env) val)
-                     (equal (satlink::eval-lit lit env) (b-xor neg val))))
-     :hints(("Goal" :in-theory (enable satlink::eval-lit))))
-
-   ;; (defthm bits-equiv-of-cnf->aignet-invals-of-aignet->cnf-vals
-   ;;   (acl2::bits-equiv (aignet::cnf->aignet-invals
-   ;;                      nil
-   ;;                      (aignet::aignet->cnf-vals
-   ;;                       invals nil nil sat-lits aignet)
-   ;;                      sat-lits aignet)
-   ;;                     (take (aignet::stype-count :pi aignet) invals))
-   ;;   :hints(("Goal" :in-theory (enable acl2::bits-equiv))))
-   ))
-
-(define logicman-bfr->cnf ((bfr lbfr-p)
-                           (logicman)
-                           (sat-lits)
-                           (cnf satlink::lit-list-listp)
-                           (cube satlink::lit-listp))
-  :guard (and (bfr-mode-is :aignet (logicman->mode logicman))
-              (b* ((index (logicman->refcounts-index logicman)))
-                (stobj-let ((aignet (logicman->aignet logicman))
-                            (u32arr (logicman->aignet-refcounts logicman)))
-                           (ok)
-                           (and (<= index (aignet::u32-length u32arr))
-                                (equal index (aignet::num-fanins aignet))
-                                (aignet::sat-lits-wfp sat-lits aignet))
-                           ok)))
-  :returns (mv new-sat-lits
-               (new-cnf satlink::lit-list-listp)
-               (new-cube satlink::lit-listp))
-  :guard-hints (("goal" :in-theory (enable logicman-invar)))
-  (b* ((lit (bfr->aignet-lit bfr (logicman->bfrstate))))
-    (stobj-let ((aignet (logicman->aignet logicman))
-                (u32arr (logicman->aignet-refcounts logicman)))
-               (sat-lits cnf cube)
-               (b* (((acl2::hintcontext-bind
-                      ((sat-lits-orig sat-lits)
-                       (cnf-orig cnf)
-                       (cube-orig cube))))
-                    ((mv sat-lits cnf)
-                     (aignet::aignet-lit->cnf lit t u32arr sat-lits aignet
-                                              (satlink::lit-list-list-fix cnf)))
-                    (sat-lit (aignet::aignet-lit->sat-lit lit sat-lits))
-                    (cube (cons sat-lit (satlink::lit-list-fix cube)))
-                    ((acl2::hintcontext :assume)))
-                 (mv sat-lits cnf cube))
-               (mv sat-lits cnf cube)))
+(define interp-st-sat-check-cube ((config fgl-satlink-monolithic-sat-config-p)
+                                  (bfr interp-st-bfr-p)
+                                  (interp-st interp-st-bfrs-ok))
+  :guard (bfr-mode-is :aignet (interp-st-bfr-mode))
+  :returns (cube satlink::lit-listp)
+  :ignore-ok t
+  :irrelevant-formals-ok t
+  ;; :guard-debug t
+  :guard-hints (("goal" :in-theory (e/d (interp-st-bfrs-ok) (not))))
+  (b* (((fgl-satlink-monolithic-sat-config config)))
+    (stobj-let ((logicman (interp-st->logicman interp-st))
+                (pathcond (interp-st->pathcond interp-st))
+                (constraint-pathcond (interp-st->constraint interp-st)))
+               (cube)
+               (b* ((cube nil)
+                    (cube
+                     (if (or** config.ignore-pathcond
+                               (not (pathcond-enabledp pathcond)))
+                         cube
+                       (pathcond-to-cube pathcond cube)))
+                    (cube
+                     (if (or** config.ignore-constraint
+                               (not (pathcond-enabledp constraint-pathcond)))
+                         cube
+                       (pathcond-to-cube constraint-pathcond cube))))
+                 (cons (bfr->aignet-lit bfr (logicman->bfrstate)) cube))
+               cube))
   ///
-  (local
-   #!aignet
-   (defthm sat-lits-wfp-implies-sat-varp-of-lookup-aignet-id-rw
-     (implies (and (bind-free '((aignet . #!fgl (logicman->aignet logicman))) (aignet))
-                   (sat-lits-wfp sat-lits aignet)
-                   (aignet-id-has-sat-var n sat-lits))
-              (sat-varp (satlink::lit->var (aignet-id->sat-lit n sat-lits))
-                        sat-lits))))
-
-  (defret sat-lits-wfp-of-<fn>
-    (implies (and (aignet::sat-lits-wfp sat-lits (logicman->aignet logicman))
-                  (lbfr-p bfr)
-                  (lbfr-mode-is :aignet))
-             (and (implies (equal aignet (logicman->aignet logicman))
-                           (aignet::sat-lits-wfp new-sat-lits aignet))
-                  (implies (aignet::sat-lit-list-listp cnf sat-lits)
-                           (aignet::sat-lit-list-listp new-cnf new-sat-lits))
-                  (implies (aignet::sat-lit-listp cube sat-lits)
-                           (aignet::sat-lit-listp new-cube new-sat-lits))))
-    :hints(("Goal" :in-theory (enable bfr-p))))
-
   
+  (local (defthm aignet-eval-conjunction-of-cons
+           (equal (aignet::aignet-eval-conjunction (cons x y) invals regvals aignet)
+                  (b-and (aignet::lit-eval x invals regvals aignet)
+                         (aignet::aignet-eval-conjunction y invals regvals aignet)))
+           :hints(("Goal" :in-theory (enable aignet::aignet-eval-conjunction)))))
 
-  (set-ignore-ok t)
+  (local (defthm aignet-eval-conjunction-of-nil
+           (equal (aignet::aignet-eval-conjunction nil invals regvals aignet)
+                  1)
+           :hints(("Goal" :in-theory (enable aignet::aignet-eval-conjunction)))))
 
-  #!aignet
-  (local (defthm lit-eval-norm-when-no-regs
-           (implies (and (syntaxp (not (equal regvals ''nil)))
-                         (equal (stype-count :reg aignet) 0))
-                    (equal (lit-eval lit invals regvals aignet)
-                           (lit-eval lit invals nil aignet)))
-           :hints (("goal" :use ((:instance lit-eval-of-take-num-regs
-                                  (n 0)))
-                    :in-theory (disable lit-eval-of-take-num-regs)))))
 
-  (defret cube-assumption-of-<fn>
-    (implies (and (aignet::sat-lits-wfp sat-lits (logicman->aignet logicman))
-                  (aignet::sat-lit-list-listp cnf sat-lits)
-                  (aignet::sat-lit-listp cube sat-lits)
-                  (aignet::cnf-for-aignet (logicman->aignet logicman)
-                                          cnf sat-lits)
+  (defret aignet-eval-conjunction-of-<fn>
+    (implies (and (equal logicman (interp-st->logicman interp-st))
+                  (equal aignet (logicman->aignet logicman))
                   (lbfr-mode-is :aignet)
-                  (equal (aignet::stype-count :reg (logicman->aignet logicman)) 0)
-                  (lbfr-p bfr)
-                  (equal (satlink::eval-formula new-cnf env) 1))
-             (equal (satlink::eval-cube new-cube env)
-                    (b* ((vals (aignet::cnf->aignet-invals
-                                nil env new-sat-lits
-                                (logicman->aignet logicman))))
-                      (b-and (satlink::eval-cube cube env)
-                             (bool->bit
-                              (bfr-eval bfr (pairlis$ (acl2::numlist 0 1 (aignet::num-ins (logicman->aignet logicman)))
-                                                      (bits->bools vals))
-                                        logicman))))))
-    :hints(("Goal" :in-theory (e/d (bfr-eval logicman-invar)
-                                   (aignet::cnf-for-aignet-implies-lit-sat-when-cnf-sat
-                                    ;; aignet::cnf-for-aignet-preserved-by-aignet-lit->cnf
-                                    ))
-            :expand ((:free (a b) (satlink::eval-cube (cons a b) env))))
-           (acl2::function-termhint
-            logicman-bfr->cnf
-            (:assume
-             `(:use ((:instance aignet::cnf-for-aignet-implies-lit-sat-when-cnf-sat
-                      (invals nil) (cnf-vals env)
-                      (sat-lits ,(acl2::hq sat-lits))
-                      (aignet ,(acl2::hq aignet))
-                      (regvals nil)
-                      (cnf ,(acl2::hq cnf))
-                      (lit ,(acl2::hq lit)))))))))
+                  ;; (equal invals (alist-to-bitarr (aignet::num-ins aignet) env nil))
+                  (logicman-pathcond-eval env
+                                          (interp-st->pathcond interp-st)
+                                          logicman)
+                  (logicman-pathcond-eval env
+                                          (interp-st->constraint interp-st)
+                                          logicman))
+               (equal (aignet::aignet-eval-conjunction
+                       cube
+                       (alist-to-bitarr (aignet::stype-count :pi aignet) env nil)
+                       ;; invals
+                       nil aignet)
+                      (bool->bit (bfr-eval bfr env))))
+    :hints(("Goal" :in-theory (enable bfr-eval))))
 
-  (defret cnf-for-aignet-of-<fn>
-    (implies (and (aignet::sat-lits-wfp sat-lits (logicman->aignet logicman))
-                  (aignet::sat-lit-list-listp cnf sat-lits)
-                  (aignet::sat-lit-listp cube sat-lits)
-                  (aignet::cnf-for-aignet (logicman->aignet logicman)
-                                          cnf sat-lits)
-                  (lbfr-mode-is :aignet)
-                  (equal (aignet::stype-count :reg (logicman->aignet logicman)) 0)
-                  (lbfr-p bfr)
-                  (equal aignet (logicman->aignet logicman)))
-             (aignet::cnf-for-aignet aignet
-                                     new-cnf new-sat-lits))
-    :hints(("Goal" :in-theory (e/d (bfr-eval logicman-invar)
-                                   (
-                                    ;; aignet::cnf-for-aignet-preserved-by-aignet-lit->cnf
-                                    )))))
+  ;; (local #!aignet
+  ;;        (defthm aignet-lit-listp-of-append
+  ;;          (implies (and (aignet-lit-listp x aignet)
+  ;;                        (aignet-lit-listp y aignet))
+  ;;                   (aignet-lit-listp (append x y) aignet))
+  ;;          :hints(("Goal" :in-theory (enable aignet-lit-listp)))))
 
-  (defret aignet-id-has-sat-var-of-<fn>
-    (implies (and (aignet::sat-lits-wfp sat-lits (logicman->aignet logicman))
-                  (aignet::sat-lit-list-listp cnf sat-lits)
-                  (aignet::sat-lit-listp cube sat-lits)
-                  (lbfr-p bfr)
-                  (lbfr-mode-is :aignet)
-                  (equal bfrstate (logicman->bfrstate)))
-             (aignet::aignet-id-has-sat-var
-              (satlink::lit->var
-               (bfr->aignet-lit bfr bfrstate))
-              new-sat-lits)))
-  
-  ;; (defret ipasir-formula-norm-of-<fn>
-  ;;   (implies (and (equal ipasir (logicman->ipasir logicman))
-  ;;                 (syntaxp (and (quotep ipasir)
-  ;;                               (equal (unquote ipasir) *logicman-empty-ipasir*))))
-  ;;            (equal
-  ;;             (ipasir::ipasir$a->formula (logicman->ipasir new-logicman))
-  ;;             (append (ipasir::ipasir$a->formula (logicman->ipasir
-  ;;                                                 (logicman-bfr->ipasir
-  ;;                                                  bfr (logicman-delete-ipasir logicman))))
-  ;;                     (ipasir::ipasir$a->formula ipasir))))
-  ;;   :hints(("Goal" :in-theory (enable logicman-delete-ipasir
-  ;;                                     logicman-update-refcounts))))
+  (local #!aignet
+         (defthm aignet-lit-listp-of-rev
+           (implies (aignet-lit-listp x aignet)
+                    (aignet-lit-listp (acl2::rev x) aignet))
+           :hints(("Goal" :in-theory (enable aignet-lit-listp acl2::rev)))))
+           
 
-  ;; (defret ipasir-assumption-norm-of-<fn>
-  ;;   (implies (and (equal ipasir (logicman->ipasir logicman))
-  ;;                 (syntaxp (and (quotep ipasir)
-  ;;                               (equal (unquote ipasir) *logicman-empty-ipasir*))))
-  ;;            (equal
-  ;;             (ipasir::ipasir$a->assumption (logicman->ipasir new-logicman))
-  ;;             (append (ipasir::ipasir$a->assumption (logicman->ipasir
-  ;;                                                    (logicman-bfr->ipasir
-  ;;                                                     bfr (logicman-delete-ipasir logicman))))
-  ;;                     (ipasir::ipasir$a->assumption ipasir))))
-  ;;   :hints(("Goal" :in-theory (enable logicman-delete-ipasir
-  ;;                                     logicman-update-refcounts))))
+  (defret aignet-lit-listp-of-<fn>
+    (implies (and (interp-st-bfrs-ok interp-st)
+                  (lbfr-mode-is :aignet (interp-st->logicman interp-st))
+                  (interp-st-bfr-p bfr))
+             (aignet::aignet-lit-listp cube (logicman->aignet (interp-st->logicman interp-st))))
+    :hints(("Goal" :in-theory (enable pathcond-to-cube
+                                      interp-st-bfrs-ok
+                                      logicman-pathcond-p)))))
 
-  ;; (defret sat-lits-norm-of-<fn>
-  ;;   (implies (and (equal ipasir (logicman->ipasir logicman))
-  ;;                 (syntaxp (and (quotep ipasir)
-  ;;                               (equal (unquote ipasir) *logicman-empty-ipasir*))))
-  ;;            (equal
-  ;;             (logicman->sat-lits new-logicman)
-  ;;             (logicman->sat-lits
-  ;;              (logicman-bfr->ipasir
-  ;;               bfr (logicman-delete-ipasir logicman)))))
-  ;;   :hints(("Goal" :in-theory (enable logicman-delete-ipasir
-  ;;                                     logicman-update-refcounts))))
 
-  (defret sat-lit-extension-p-of-<fn>
-    (aignet::sat-lit-extension-p new-sat-lits sat-lits)))
 
 (encapsulate
-  (((fgl-satlink-config) => *))
+  (((fgl-satlink-config) => *
+    :formals nil :guard t))
   (local (defun fgl-satlink-config ()
+           (declare (xargs :guard t))
            satlink::*default-config*))
   (defthm fgl-satlink-config-constraint
     (satlink::config-p (fgl-satlink-config))))
@@ -287,48 +147,37 @@
 
 (defattach fgl-satlink-config fgl-default-satlink-config)
 
-(define cnf-assume-cube ((cube satlink::lit-listp)
-                         (cnf satlink::lit-list-listp))
-  :returns (new-cnf satlink::lit-list-listp)
-  (if (atom cube)
-      (satlink::lit-list-list-fix cnf)
-    (cnf-assume-cube
-     (cdr cube)
-     (cons (list (satlink::lit-fix (car cube)))
-           (satlink::lit-list-list-fix cnf))))
-  ///
-  (defthm eval-of-cnf-assume-cube
-    (equal (satlink::eval-formula (cnf-assume-cube cube cnf) env)
-           (b-and (satlink::eval-cube cube env)
-                  (satlink::eval-formula cnf env)))
-    :hints(("Goal" :in-theory (enable satlink::eval-formula satlink::eval-cube satlink::eval-clause)))))
+(define fgl-satlink-config-wrapper ((x fgl-satlink-monolithic-sat-config-p))
+  :returns (config satlink::config-p)
+  (b* ((config-config (fgl-satlink-monolithic-sat-config->satlink-config-override x))
+       ((when (and config-config (satlink::config-p config-config)))
+        config-config))
+    (fgl-satlink-config)))
 
 
-(local (include-book "tools/trivial-ancestors-check" :dir :system))
-(local (acl2::use-trivial-ancestors-check))
+(encapsulate
+  (((fgl-aignet-transforms-config) => *
+    :formals nil :guard t))
+  (local (defun fgl-aignet-transforms-config ()
+           (declare (xargs :guard t))
+           nil)))
 
-(local (defcong logicman-equiv equal (logicman-extension-p new old) 1
-         :hints(("Goal" :in-theory (enable logicman-equiv logicman-extension-p)))))
+(defun fgl-default-aignet-transforms-config ()
+  (declare (xargs :guard t))
+  nil)
 
-(local (defthm logicman-extension-p-when-logicman-equiv
-         (implies (logicman-equiv (double-rewrite new) old)
-                  (logicman-extension-p new old))))
+(defattach fgl-aignet-transforms-config fgl-default-aignet-transforms-config)
 
-(local (defthm logicman-update-refcounts-preserves-logicman-invar
-         (implies (logicman-invar logicman)
-                  (logicman-invar (logicman-update-refcounts logicman)))
-         :hints(("Goal" :in-theory (enable logicman-invar)))))
+(define fgl-aignet-transforms-config-wrapper ((x fgl-satlink-monolithic-sat-config-p))
+  (b* ((config-config (fgl-satlink-monolithic-sat-config->transform-config-override x)))
+    (or config-config
+        (fgl-aignet-transforms-config))))
 
-(local (defthm logicman-pathcond-to-cnf-preserves-logicman-invar
-         (implies (logicman-invar logicman)
-                  (logicman-invar (mv-nth 0 (logicman-pathcond-to-cnf pathcond logicman sat-lits cnf cube))))
-         :hints(("Goal" :in-theory (enable logicman-invar logicman-pathcond-to-cnf)))))
 
-(local (in-theory (disable resize-list
-                           lrat::nth-n59-listp
-                           lrat::nth-i60-listp)))
 
-(define interp-st-satlink-sat-check-core ((config fgl-sat-config-p)
+
+
+(define interp-st-satlink-sat-check-core ((config fgl-satlink-monolithic-sat-config-p)
                                           (bfr interp-st-bfr-p)
                                           (interp-st interp-st-bfrs-ok)
                                           state)
@@ -341,52 +190,28 @@
   :guard-hints (("goal" :in-theory (e/d (interp-st-bfrs-ok) (not))))
   (b* (((unless (bfr-mode-is :aignet (interp-st-bfr-mode)))
         (mv bfr interp-st))
-       ((fgl-sat-config config)))
+       (cube (interp-st-sat-check-cube config bfr interp-st))
+       ((fgl-satlink-monolithic-sat-config config)))
     (stobj-let ((logicman (interp-st->logicman interp-st))
-                (pathcond (interp-st->pathcond interp-st))
-                (constraint-pathcond (interp-st->constraint interp-st))
                 (env$ (interp-st->ctrex-env interp-st)))
-               (ans logicman env$)
-               (b* (((acl2::local-stobjs sat-lits satlink::env$)
-                     (mv ans logicman env$ sat-lits satlink::env$))
-                    (cnf nil)
-                    (cube nil)
-                    (num-fanins (stobj-let ((aignet (logicman->aignet logicman)))
-                                           (num-fanins)
-                                           (aignet::num-fanins aignet)
-                                           num-fanins))
-                    (sat-lits (resize-aignet->sat num-fanins sat-lits))
-                    ((mv logicman sat-lits cnf cube)
-                     (if (or** config.ignore-pathcond
-                               (not (pathcond-enabledp pathcond)))
-                         (mv logicman sat-lits cnf cube)
-                       (logicman-pathcond-to-cnf pathcond logicman sat-lits cnf cube)))
-                    ((mv logicman sat-lits cnf cube)
-                     (if (or** config.ignore-constraint
-                               (not (pathcond-enabledp constraint-pathcond)))
-                         (mv logicman sat-lits cnf cube)
-                       (logicman-pathcond-to-cnf constraint-pathcond logicman sat-lits cnf cube)))
-                    (logicman (logicman-update-refcounts logicman))
-                    ((mv sat-lits cnf cube)
-                     (logicman-bfr->cnf bfr logicman sat-lits cnf cube))
-                    (cnf (cnf-assume-cube cube cnf))
-                    (config  (fgl-satlink-config))
-                    ;; ((acl2::hintcontext-bind ((logicman-solve logicman))))
-                    ((acl2::hintcontext :solve))
-                    ((mv ans satlink::env$) (satlink::sat cnf satlink::env$ :config config))
-                    (env$
-                     (stobj-let ((bitarr (env$->bitarr env$)))
-                                (bitarr)
-                                (stobj-let ((aignet (logicman->aignet logicman)))
-                                           (bitarr)
-                                           (b* ((bitarr (resize-bits (aignet::num-fanins aignet) bitarr)))
-                                             (aignet::cnf->aignet-vals bitarr satlink::env$ sat-lits aignet))
-                                           bitarr)
-                                env$)))
-                 (mv ans logicman env$ sat-lits satlink::env$))
-               (if (eq ans :unsat)
-                   (mv nil interp-st)
-                 (mv bfr interp-st))))
+               (ans env$)
+               (stobj-let ((aignet (logicman->aignet logicman)))
+                          (ans env$)
+                          (stobj-let ((bitarr (env$->bitarr env$)))
+                                     (ans bitarr)
+                                     (b* ((satlink-config (fgl-satlink-config-wrapper config))
+                                          
+                                          ((unless config.transform)
+                                           (acl2::hintcontext
+                                            :no-xform
+                                            (aignet::aignet-sat-check-cube cube satlink-config aignet bitarr)))
+                                          (transform-config (fgl-aignet-transforms-config-wrapper config))
+                                          ((acl2::hintcontext :xform)))
+                                       (aignet::aignet-transform-sat-check-cube
+                                        cube satlink-config transform-config aignet bitarr))
+                                     (mv (if (eq ans :unsat) nil bfr) env$))
+                          (mv ans env$))
+               (mv ans interp-st)))
   ///
   
   (defret interp-st-bfrs-ok-of-<fn>
@@ -406,232 +231,7 @@
                     (interp-st->logicman interp-st))
     :hints(("Goal" :in-theory (enable logicman-equiv))))
 
-  (local
-   #!aignet
-   (defthm aignet-eval-conjunction-of-nil
-     (equal (aignet-eval-conjunction nil invals regvals aignet) 1)
-     :hints(("Goal" :in-theory (enable aignet-eval-conjunction)))))
-  
-  #!aignet
-  (local (defthm lit-eval-norm-when-no-regs
-           (implies (and (syntaxp (not (equal regvals ''nil)))
-                         (equal (stype-count :reg aignet) 0))
-                    (equal (lit-eval lit invals regvals aignet)
-                           (lit-eval lit invals nil aignet)))
-           :hints (("goal" :use ((:instance lit-eval-of-take-num-regs
-                                  (n 0)))
-                    :in-theory (disable lit-eval-of-take-num-regs)))))
-
-
-  (local
-   #!aignet
-   (defthm cnf-for-aignet-implies-lit-sat-when-cnf-sat-rw
-     (b* ((invals (cnf->aignet-invals invals cnf-vals satlits aignet))
-          (regvals nil))
-       (implies (and (sat-lits-wfp satlits aignet)
-                     (bind-free
-                      (case-match satlits
-                        (('mv-nth ''0 ('fgl::logicman-bfr->cnf . args))
-                         `((cnf . (mv-nth '1 (fgl::logicman-bfr->cnf . ,args)))))
-                        (& (cw "satlits: ~x0~%" satlits)))
-                      
-                      (cnf))
-                     (cnf-for-aignet aignet cnf satlits)
-                     (aignet-litp lit aignet)
-                     (aignet-id-has-sat-var (lit-id lit) satlits)
-                     (equal 1 (satlink::eval-formula cnf cnf-vals))
-                     (equal (stype-count :reg aignet) 0))
-                (equal (lit-eval lit invals regvals aignet)
-                       (satlink::eval-lit
-                        (aignet-lit->sat-lit lit satlits)
-                        cnf-vals))))
-     :hints (("goal" :use ((:instance cnf-for-aignet-implies-lit-sat-when-cnf-sat
-                            (sat-lits satlits)))
-              :in-theory (disable cnf-for-aignet-implies-lit-sat-when-cnf-sat)))))
-
-  (local (in-theory (disable aignet::aignet-lit->sat-lit)))
-
-  (local
-   #!aignet
-   (acl2::def-updater-independence-thm eval-conjunction-in-aignet->cnf-vals-of-sat-lit-extension-logicman
-     (implies (and (sat-lit-extension-p (fgl::logicman->sat-lits new)
-                                        (fgl::logicman->sat-lits old))
-                   (sat-lit-listp conjunction (fgl::logicman->sat-lits old)))
-              (equal (eval-cube
-                      conjunction (aignet->cnf-vals
-                                   invals regvals cnf-vals
-                                   (fgl::logicman->sat-lits new) aignet))
-                     (eval-cube
-                      conjunction (aignet->cnf-vals
-                                   invals regvals cnf-vals
-                                   (fgl::logicman->sat-lits old) aignet))))))
-
-  (local
-   #!aignet
-   (acl2::def-updater-independence-thm nbalist-has-sat-lits-of-sat-lit-extension-logicman
-     (implies (and (sat-lit-extension-p (fgl::logicman->sat-lits new)
-                                        (fgl::logicman->sat-lits old))
-                   (nbalist-has-sat-lits nbalist (fgl::logicman->sat-lits old)))
-              (nbalist-has-sat-lits nbalist (fgl::logicman->sat-lits new)))))
-
-  (local
-   #!aignet
-   (defthm cnf-for-aignet-implies-cnf-sat-when-lit-sat-rw
-     (b* ((cnf-vals (aignet->cnf-vals
-                     invals regvals cnf-vals sat-lits aignet)))
-       (implies (and (sat-lits-wfp sat-lits aignet)
-                     (bind-free
-                      (case-match sat-lits
-                        (('mv-nth ''0 ('fgl::logicman-bfr->cnf . args))
-                         `((cnf . (mv-nth '1 (fgl::logicman-bfr->cnf . ,args)))))
-                        (& nil))
-                      (cnf))
-                     (cnf-for-aignet aignet cnf sat-lits)
-                     (aignet-litp lit aignet)
-                     (aignet-id-has-sat-var (lit-id lit) sat-lits))
-                (equal (satlink::eval-lit
-                        (aignet-lit->sat-lit lit sat-lits)
-                        cnf-vals)
-                       (lit-eval lit invals regvals aignet)
-                       ;; (lit-eval lit invals regvals aignet)
-                       )))))
-
-  (local
-   #!aignet
-   (defthm cnf-for-aignet-implies-eval-formula
-     (implies (cnf-for-aignet aignet cnf sat-lits)
-              (equal (satlink::eval-formula
-                      cnf (aignet->cnf-vals invals regvals cnf-vals sat-lits aignet))
-                     1))))
-
-
-  (local (in-theory (disable aignet::eval-cube-of-aignet->cnf-vals)))
-
-  (local (defthm eval-cube-of-nil
-           (equal (satlink::eval-cube nil env) 1)
-           :hints(("Goal" :in-theory (enable satlink::eval-cube)))))
-
-
-  #!aignet
-  (local (defthm aignet-pathcond-eval-norm-when-no-regs
-           (implies (and (syntaxp (not (equal regvals ''nil)))
-                         (equal (stype-count :reg aignet) 0))
-                    (iff (aignet-pathcond-eval aignet pathcond invals regvals)
-                         (aignet-pathcond-eval aignet pathcond invals nil)))
-           :hints ((and stable-under-simplificationp
-                        (let* ((lit (assoc 'aignet-pathcond-eval clause))
-                               (other (if (eq (car (last lit)) 'regvals)
-                                          nil
-                                        'regvals)))
-                          `(:expand (,lit)
-                            :use ((:instance aignet-pathcond-eval-necc
-                                   (id (aignet-pathcond-eval-witness . ,(cdr lit)))
-                                   (nbalist pathcond)
-                                   (regvals ,other)))
-                            :do-not-induct t))))))
-
-  (local
-   #!aignet
-   (defthm cnf-for-aignet-implies-aignet-pathcond-eval-when-cnf-sat-no-regs
-     (b* ((invals (cnf->aignet-invals invals cnf-vals sat-lits aignet))
-          (regvals nil))
-       (implies (and (sat-lits-wfp sat-lits aignet)
-                     (bind-free
-                      (case-match sat-lits
-                        (('mv-nth ''0 ('fgl::logicman-bfr->cnf . args))
-                         `((cnf . (mv-nth '1 (fgl::logicman-bfr->cnf . ,args)))))
-                        (('mv-nth ''1 ('fgl::logicman-pathcond-to-cnf . args))
-                         `((cnf . (mv-nth '2 (fgl::logicman-pathcond-to-cnf . ,args)))))
-                        (& nil))
-                      (cnf))
-                     (cnf-for-aignet aignet cnf sat-lits)
-                     (aignet-pathcond-p nbalist aignet)
-                     (nbalist-has-sat-lits nbalist sat-lits)
-                     (equal 1 (satlink::eval-formula cnf cnf-vals))
-                     (equal (stype-count :reg aignet) 0))
-                (equal (aignet-pathcond-eval aignet nbalist invals regvals)
-                       (bit->bool (satlink::eval-cube
-                                   (nbalist-to-cube nbalist sat-lits)
-                                   cnf-vals)))))
-     :hints(("Goal" :use cnf-for-aignet-implies-aignet-pathcond-eval-when-cnf-sat
-             :in-theory (disable cnf-for-aignet-implies-aignet-pathcond-eval-when-cnf-sat)))))
-
-  (local (defthm aignet-pathcond-p-when-logicman-pathcond-p
-           (implies (and (logicman-pathcond-p pathcond logicman)
-                         (lbfr-mode-is :aignet))
-                    (aignet::aignet-pathcond-p (nth *pathcond-aignet* pathcond) 
-                                               (logicman->aignet logicman)))
-           :hints(("Goal" :in-theory (enable logicman-pathcond-p)))))
-
-  (local
-   #!aignet
-   (defthm bitp-cdar-of-nbalist-fix
-     (implies (consp (nbalist-fix x))
-              (Bitp (cdar (nbalist-fix x))))
-     :hints(("Goal" :in-theory (enable nbalist-fix)))
-     :rule-classes :type-prescription))
-
-  (local
-   #!aignet
-   (defthm cnf-for-aignet-implies-eval-nbalist-to-cube-of-aignet->cnf-vals-lemma
-     (b* ((cnf-vals (aignet->cnf-vals
-                     invals regvals cnf-vals sat-lits aignet)))
-       (implies (and (sat-lits-wfp sat-lits aignet)
-                     (bind-free
-                      (case-match sat-lits
-                        (('mv-nth ''0 ('fgl::logicman-bfr->cnf . args))
-                         `((cnf . (mv-nth '1 (fgl::logicman-bfr->cnf . ,args)))))
-                        (('mv-nth ''1 ('fgl::logicman-pathcond-to-cnf . args))
-                         `((cnf . (mv-nth '2 (fgl::logicman-pathcond-to-cnf . ,args)))))
-                        (& nil))
-                      (cnf))
-                     (cnf-for-aignet aignet cnf sat-lits)
-                     (aignet-pathcond-p nbalist aignet)
-                     (nbalist-has-sat-lits nbalist sat-lits))
-                (equal (satlink::eval-cube
-                        (nbalist-to-cube nbalist sat-lits)
-                        cnf-vals)
-                       (bool->bit (aignet-pathcond-eval aignet nbalist invals regvals))
-                       ;; (lit-eval lit invals regvals aignet)
-                       )))
-     :hints(("Goal" :in-theory (enable nbalist-has-sat-lits
-                                       aignet-pathcond-p-redef
-                                       aignet-pathcond-eval-redef
-                                       nbalist-to-cube
-                                       eval-cube
-                                       lit-eval)))))
-
-  (local
-   #!aignet
-   (defthm cnf-for-aignet-implies-eval-nbalist-to-cube-of-aignet->cnf-vals
-     (b* ((cnf-vals (aignet->cnf-vals
-                     invals regvals cnf-vals sat-lits aignet)))
-       (implies (and (sat-lits-wfp sat-lits aignet)
-                     (bind-free
-                      (case-match sat-lits
-                        (('mv-nth ''0 ('fgl::logicman-bfr->cnf . args))
-                         `((cnf . (mv-nth '1 (fgl::logicman-bfr->cnf . ,args)))))
-                        (('mv-nth ''1 ('fgl::logicman-pathcond-to-cnf . args))
-                         `((cnf . (mv-nth '2 (fgl::logicman-pathcond-to-cnf . ,args)))))
-                        (& nil))
-                      (cnf))
-                     (cnf-for-aignet aignet cnf sat-lits)
-                     (aignet-pathcond-p nbalist aignet)
-                     (nbalist-has-sat-lits nbalist sat-lits1)
-                     (aignet::sat-lit-extension-p sat-lits sat-lits1))
-                (equal (satlink::eval-cube
-                        (nbalist-to-cube nbalist sat-lits1)
-                        cnf-vals)
-                       (bool->bit (aignet-pathcond-eval aignet nbalist invals regvals))
-                       ;; (lit-eval lit invals regvals aignet)
-                       )))
-     :hints(("Goal" :use ((:instance cnf-for-aignet-implies-eval-nbalist-to-cube-of-aignet->cnf-vals-lemma))
-             :in-theory (disable cnf-for-aignet-implies-eval-nbalist-to-cube-of-aignet->cnf-vals-lemma)))))
-
   (set-ignore-ok t)
-
-  (local (in-theory (disable b-and)))
-
   (defret eval-of-<fn>
     (implies (and (interp-st-bfrs-ok interp-st)
                   (interp-st-bfr-p bfr)
@@ -647,27 +247,32 @@
                     (gobj-bfr-eval bfr env (interp-st->logicman interp-st))))
     :hints ((acl2::function-termhint
              interp-st-satlink-sat-check-core
-             (:solve
-              (b* ((aignet (logicman->aignet logicman))
-                   (aignet-invals (alist-to-bitarr (aignet::num-ins aignet)
-                                                   (gl-env->bfr-vals env) nil))
-                   (cnf-vals (aignet::aignet->cnf-vals aignet-invals nil nil sat-lits aignet)))
-                `(:use ((:instance satlink::sat-when-unsat
-                         (formula ,(acl2::hq cnf))
-                         (env ,(acl2::hq cnf-vals))
-                         (config ,(acl2::hq config))
-                        ;; (:instance aignet::cnf-for-aignet-implies-eval-formula
-                        ;;  (cnf ,(acl2::hq (ipasir::ipasir$a->formula ipasir)))
-                        ;;  (invals ,(acl2::hq aignet-invals))
-                        ;;  (regvals nil)
-                        ;;  (cnf-vals nil)
-                        ;;  (sat-lits ,(acl2::hq sat-lits))
-                        ;;  (aignet ,(acl2::hq aignet)))
-                        ))
-                  :in-theory (e/d (bfr-eval logicman-pathcond-eval)
-                                  ;; (aignet::cnf-for-aignet-necc
-                                  ;;  aignet::cnf-for-aignet-implies-eval-formula)
-                                  )))))))
+             (:no-xform
+              (b* ((invals (alist-to-bitarr (aignet::num-ins aignet)
+                                            (gl-env->bfr-vals env) nil)))
+                `(:in-theory (e/d (gobj-bfr-eval bfr-eval)
+                                  (aignet::aignet-sat-check-cube-unsat))
+                  :use ((:instance aignet::aignet-sat-check-cube-unsat
+                         (cube ,(acl2::hq cube))
+                         (config ,(acl2::hq satlink-config))
+                         (aignet ,(acl2::hq aignet))
+                         (bitarr ,(acl2::hq bitarr))
+                         (invals ,(acl2::hq invals))
+                         (regvals nil))))))
+             (:xform
+              (b* ((invals (alist-to-bitarr (aignet::num-ins aignet)
+                                            (gl-env->bfr-vals env) nil)))
+                `(:in-theory (e/d (gobj-bfr-eval bfr-eval)
+                                  (aignet::aignet-transform-sat-check-cube-unsat))
+                  :use ((:instance aignet::aignet-transform-sat-check-cube-unsat
+                         (cube ,(acl2::hq cube))
+                         (sat-config ,(acl2::hq satlink-config))
+                         (xform-config ,(acl2::hq transform-config))
+                         (aignet ,(acl2::hq aignet))
+                         (bitarr ,(acl2::hq bitarr))
+                         (invals ,(acl2::hq invals))
+                         (regvals nil)))))))))
+                                
   
 
 
@@ -692,27 +297,6 @@
     (equal (bfr-nvars (interp-st->logicman new-interp-st))
            (bfr-nvars (interp-st->logicman interp-st))))
 
-  ;; (defret pathcond-eval-checkpoints-of-<fn>
-  ;;   (implies (equal pathcond (interp-st->pathcond interp-st))
-  ;;            (equal (logicman-pathcond-eval-checkpoints!
-  ;;                    env
-  ;;                    pathcond
-  ;;                    (interp-st->logicman new-interp-st))
-  ;;                   (logicman-pathcond-eval-checkpoints!
-  ;;                    env
-  ;;                    pathcond
-  ;;                    (interp-st->logicman interp-st)))))
-
-  ;;   (defret constraint-eval-of-<fn>
-  ;;     (implies (equal constraint (interp-st->constraint interp-st))
-  ;;              (equal (logicman-pathcond-eval
-  ;;                      env
-  ;;                      constraint
-  ;;                      (interp-st->logicman new-interp-st))
-  ;;                     (logicman-pathcond-eval
-  ;;                      env
-  ;;                      constraint
-  ;;                      (interp-st->logicman interp-st)))))
   
   (defret <fn>-return-values-correct
     (equal (list . <values>)
@@ -724,20 +308,10 @@
                (equal (interp-st->errmsg new-interp-st) errmsg))))
 
   
-  
-  ;; (defret get-bvar->term-eval-of-<fn>
-  ;;   (implies (equal bvar-db (interp-st->bvar-db interp-st))
-  ;;            (iff (fgl-object-eval (get-bvar->term$a n bvar-db)
-  ;;                                  env
-  ;;                                  (interp-st->logicman new-interp-st))
-  ;;                 (fgl-object-eval (get-bvar->term$a n bvar-db)
-  ;;                                  env
-  ;;                                  (interp-st->logicman interp-st)))))
 
   (defret interp-st->errmsg-equal-unreachable-of-<fn>
     (implies (not (equal (interp-st->errmsg interp-st) :unreachable))
              (not (equal (interp-st->errmsg new-interp-st) :unreachable)))))
-
 
 (make-event
  `(define interp-st-satlink-sat-check-impl (params
@@ -751,7 +325,7 @@
           (mv bfr interp-st))
          ((when (interp-st->errmsg interp-st))
           (mv nil interp-st))
-         ((unless (fgl-sat-config-p params))
+         ((unless (fgl-satlink-monolithic-sat-config-p params))
           (gl-interp-error
            :msg (gl-msg "Malformed fgl-sat-check call: params was not resolved to a fgl-sat-config object"))))
       (interp-st-satlink-sat-check-core params bfr interp-st state))
@@ -808,8 +382,16 @@
              (bfr-env$-p (interp-st->ctrex-env new-interp-st)
                          (logicman->bfrstate (interp-st->logicman interp-st))))))
 
+
+(make-event
+ `(define fgl-satlink-default-toplevel-sat-check-config ()
+    ',(make-fgl-satlink-monolithic-sat-config :ignore-pathcond nil)))
+
 (defmacro fgl-use-satlink-for-monolithic-sat ()
   '(progn (defattach interp-st-monolithic-sat-check interp-st-satlink-sat-check-impl)
-          (defattach interp-st-monolithic-sat-counterexample interp-st-satlink-counterexample)))
+          (defattach interp-st-monolithic-sat-counterexample interp-st-satlink-counterexample)
+          (defattach fgl-toplevel-sat-check-config fgl-satlink-default-toplevel-sat-check-config)))
 
 (fgl-use-satlink-for-monolithic-sat)
+
+
