books/centaur/fgl/tests.lisp
@@ -35,7 +35,7 @@
 
 (include-book "centaur/ipasir/ipasir-backend" :dir :system)
 
-
+(value-triple (acl2::tshell-ensure))
 
 
 
@@ -59,58 +59,55 @@
             (or (not (a)) (not (b)) (not (c)))))
   :hints (("goal" :clause-processor (gl-interp-cp clause
                                                       (default-glcp-config)
-                                                      state))))
+                                                      interp-st state))))
 
 
 
-(include-book "centaur/bitops/ihsext-basics" :dir :system)
+;; (include-book "centaur/bitops/ihsext-basics" :dir :system)
 
-(def-gl-rewrite unsigned-byte-p-means-equal-loghead
-  (implies (natp n)
-           (iff (unsigned-byte-p n x)
-                (equal x (loghead n x)))))
+;; (def-gl-rewrite unsigned-byte-p-means-equal-loghead
+;;   (implies (natp n)
+;;            (iff (unsigned-byte-p n x)
+;;                 (equal x (loghead n x)))))
 
-(def-gl-rewrite loghead-expand
-  (implies (syntaxp (natp n))
-           (equal (loghead n x)
-                  (if (zp n)
-                      0
-                    (intcons (and (intcar x) t)
-                             (loghead (1- n) (intcdr x))))))
-  :hints(("Goal" :in-theory (enable intcons intcar intcdr
-                                    bitops::loghead**))))
+;; (def-gl-rewrite loghead-expand
+;;   (implies (syntaxp (natp n))
+;;            (equal (loghead n x)
+;;                   (if (zp n)
+;;                       0
+;;                     (intcons (and (intcar x) t)
+;;                              (loghead (1- n) (intcdr x))))))
+;;   :hints(("Goal" :in-theory (enable intcons intcar intcdr
+;;                                     bitops::loghead**))))
 
-(def-gl-rewrite logtail-def
-  (implies (syntaxp (natp n))
-           (equal (logtail n x)
-                  (if (zp n)
-                      (int x)
-                    (logtail (1- n) (intcdr x)))))
-  :hints(("Goal" :in-theory (enable int intcdr bitops::logtail**))))
-
-
+;; (def-gl-rewrite logtail-def
+;;   (implies (syntaxp (natp n))
+;;            (equal (logtail n x)
+;;                   (if (zp n)
+;;                       (int x)
+;;                     (logtail (1- n) (intcdr x)))))
+;;   :hints(("Goal" :in-theory (enable int intcdr bitops::logtail**))))
 
 
-(table gl-fn-modes
-       nil
-       (let ((my-fn-mode (make-gl-function-mode :dont-expand-def t)))
 
-         (list (cons 'unsigned-byte-p my-fn-mode)
-               (cons 'acl2::loghead$inline my-fn-mode)
-               (cons 'acl2::logtail$inline my-fn-mode)
-               (cons 'intcdr my-fn-mode)
-               (cons 'intcar my-fn-mode)
-               (cons 'int my-fn-mode)
-               (cons 'intcons my-fn-mode))) :clear)
+
+;; (table gl-fn-modes
+;;        nil
+;;        (let ((my-fn-mode (make-gl-function-mode :dont-expand-def t)))
+
+;;          (list (cons 'unsigned-byte-p my-fn-mode)
+;;                (cons 'acl2::loghead$inline my-fn-mode)
+;;                (cons 'acl2::logtail$inline my-fn-mode)
+;;                (cons 'intcdr my-fn-mode)
+;;                (cons 'intcar my-fn-mode)
+;;                (cons 'int my-fn-mode)
+;;                (cons 'intcons my-fn-mode))) :clear)
 
 
   
-(thm
- (if (unsigned-byte-p 5 x)
-     (equal (logtail 7 x) 0)
-   t)
- :hints (("goal" :clause-processor (gl-interp-cp clause (default-glcp-config) state)
-          :in-theory nil)))
+(fgl-thm
+ :hyp (unsigned-byte-p 5 x)
+ :concl (equal (logtail 7 x) 0))
 
 
 ;; (def-gl-rewrite fgl-logand-of-ends
@@ -126,31 +123,31 @@
 ;;      (check-int-endp-fn x xsyn)))
 
 
-(def-gl-rewrite fgl-logand
-  (equal (logand x y)
-         (b* ((x (int x))
-              (y (int y))
-              (xsyn (syntax-bind xsyn (g-concrete x)))
-              (ysyn (syntax-bind ysyn (g-concrete y)))
-              ((when (and (check-int-endp x xsyn)
-                          (check-int-endp y ysyn)))
-               (endint (and (intcar x)
-                            (intcar y)))))
-           (intcons (and (intcar x)
-                         (intcar y))
-                    (logand (intcdr x) (intcdr y)))))
-  :hints(("Goal" :in-theory (enable bitops::logand** int-endp))))
+;; (def-gl-rewrite fgl-logand
+;;   (equal (logand x y)
+;;          (b* ((x (int x))
+;;               (y (int y))
+;;               (xsyn (syntax-bind xsyn (g-concrete x)))
+;;               (ysyn (syntax-bind ysyn (g-concrete y)))
+;;               ((when (and (check-int-endp x xsyn)
+;;                           (check-int-endp y ysyn)))
+;;                (endint (and (intcar x)
+;;                             (intcar y)))))
+;;            (intcons (and (intcar x)
+;;                          (intcar y))
+;;                     (logand (intcdr x) (intcdr y)))))
+;;   :hints(("Goal" :in-theory (enable bitops::logand** int-endp))))
 
 
-(def-gl-rewrite fgl-integerp-of-int
-  (integerp (int x)))
+;; (def-gl-rewrite fgl-integerp-of-int
+;;   (integerp (int x)))
 
-(def-gl-rewrite fgl-consp-of-cons
-  (consp (cons x y)))
+;; (def-gl-rewrite fgl-consp-of-cons
+;;   (consp (cons x y)))
 
 
-(def-gl-rewrite fgl-booleanp-of-bool
-  (booleanp (bool x)))
+;; (def-gl-rewrite fgl-booleanp-of-bool
+;;   (booleanp (bool x)))
 
 
 
@@ -183,81 +180,81 @@
 ;;   (equal (equal (endint x) (endint y))
 ;;          (iff x y)))
 
-(def-gl-rewrite integerp-int
-  (integerp (int x)))
+;; (def-gl-rewrite integerp-int
+;;   (integerp (int x)))
 
-(def-gl-rewrite integerp-bool
-  (not (integerp (bool x))))
+;; (def-gl-rewrite integerp-bool
+;;   (not (integerp (bool x))))
 
-(def-gl-rewrite integerp-cons
-  (not (integerp (cons x y))))
+;; (def-gl-rewrite integerp-cons
+;;   (not (integerp (cons x y))))
 
-(def-gl-rewrite consp-cons
-  (consp (cons x y)))
+;; (def-gl-rewrite consp-cons
+;;   (consp (cons x y)))
 
-(def-gl-rewrite consp-int
-  (not (consp (int x))))
+;; (def-gl-rewrite consp-int
+;;   (not (consp (int x))))
 
-(def-gl-rewrite consp-bool
-  (not (consp (bool x))))
+;; (def-gl-rewrite consp-bool
+;;   (not (consp (bool x))))
 
-(def-gl-rewrite booleanp-bool
-  (booleanp (bool x)))
+;; (def-gl-rewrite booleanp-bool
+;;   (booleanp (bool x)))
 
-(def-gl-rewrite booleanp-int
-  (not (booleanp (int x))))
+;; (def-gl-rewrite booleanp-int
+;;   (not (booleanp (int x))))
 
-(def-gl-rewrite booleanp-cons
-  (not (booleanp (cons x y))))
-
-
-(define check-integerp (x xsyn)
-  :verify-guards nil
-  (and (gobj-syntactic-integerp xsyn)
-       (integerp x))
-  ///
-  (defthm check-integerp-open
-    (iff (check-integerp x xsyn)
-         (and* (gobj-syntactic-integerp xsyn)
-               (integerp x)))))
+;; (def-gl-rewrite booleanp-cons
+;;   (not (booleanp (cons x y))))
 
 
+;; (define check-integerp (x xsyn)
+;;   :verify-guards nil
+;;   (and (gobj-syntactic-integerp xsyn)
+;;        (integerp x))
+;;   ///
+;;   (defthm check-integerp-open
+;;     (iff (check-integerp x xsyn)
+;;          (and* (gobj-syntactic-integerp xsyn)
+;;                (integerp x)))))
 
 
 
 
 
-(def-gl-rewrite fgl-equal
-  (equal (equal x y)
-         (let ((xsyn (syntax-bind xsyn (g-concrete x)))
-               (ysyn (syntax-bind ysyn (g-concrete y))))
-           (cond ((check-integerp x xsyn)
-                  (cond ((check-integerp y ysyn)
-                         (and (iff (intcar x) (intcar y))
-                              (or (and (check-int-endp x xsyn)
-                                       (check-int-endp y ysyn))
-                                  (equal (intcdr x) (intcdr y)))))
-                        ((check-non-integerp y ysyn) nil)
-                        (t (abort-rewrite (equal x y)))))
-                 ((check-booleanp x xsyn)
-                  (cond ((check-booleanp y ysyn)
-                         (iff x y))
-                        ((check-non-booleanp y ysyn) nil)
-                        (t (abort-rewrite (equal x y)))))
-                 ((check-consp x xsyn)
-                  (cond ((check-consp y ysyn)
-                         (and (equal (car x) (car y))
-                              (equal (cdr x) (cdr y))))
-                        ((check-non-consp y ysyn) nil)
-                        (t (abort-rewrite (equal x y)))))
-                 ((and (check-integerp y ysyn)
-                       (check-non-integerp x xsyn)) nil)
-                 ((and (check-booleanp y ysyn)
-                       (check-non-booleanp x xsyn)) nil)
-                 ((and (check-consp y ysyn)
-                       (check-non-consp x xsyn)) nil)
-                 (t (abort-rewrite (equal x y))))))
-  :hints(("Goal" :in-theory (enable int-endp))))
+
+
+;; (def-gl-rewrite fgl-equal
+;;   (equal (equal x y)
+;;          (let ((xsyn (syntax-bind xsyn (g-concrete x)))
+;;                (ysyn (syntax-bind ysyn (g-concrete y))))
+;;            (cond ((check-integerp x xsyn)
+;;                   (cond ((check-integerp y ysyn)
+;;                          (and (iff (intcar x) (intcar y))
+;;                               (or (and (check-int-endp x xsyn)
+;;                                        (check-int-endp y ysyn))
+;;                                   (equal (intcdr x) (intcdr y)))))
+;;                         ((check-non-integerp y ysyn) nil)
+;;                         (t (abort-rewrite (equal x y)))))
+;;                  ((check-booleanp x xsyn)
+;;                   (cond ((check-booleanp y ysyn)
+;;                          (iff x y))
+;;                         ((check-non-booleanp y ysyn) nil)
+;;                         (t (abort-rewrite (equal x y)))))
+;;                  ((check-consp x xsyn)
+;;                   (cond ((check-consp y ysyn)
+;;                          (and (equal (car x) (car y))
+;;                               (equal (cdr x) (cdr y))))
+;;                         ((check-non-consp y ysyn) nil)
+;;                         (t (abort-rewrite (equal x y)))))
+;;                  ((and (check-integerp y ysyn)
+;;                        (check-non-integerp x xsyn)) nil)
+;;                  ((and (check-booleanp y ysyn)
+;;                        (check-non-booleanp x xsyn)) nil)
+;;                  ((and (check-consp y ysyn)
+;;                        (check-non-consp x xsyn)) nil)
+;;                  (t (abort-rewrite (equal x y))))))
+;;   :hints(("Goal" :in-theory (enable int-endp))))
                
                      
                      
@@ -285,39 +282,38 @@
 ;; (def-gl-rewrite fgl-equal-bools
 ;;   (equal (equal (bool x) (bool y))
 ;;          (iff x y)))
+(make-event
+ (er-progn (assign :fgl-trace-rewrites t)
+           (assign :fgl-trace-rule-alist '(((:rewrite loghead-const-width))
+                                           ((:rewrite loghead-to-logmask-helper))
+                                           ((:rewrite fgl-equal))))
+           (value '(value-triple :trace-on))))
+
+(fgl-thm
+ :hyp (and (unsigned-byte-p 5 x)
+           (unsigned-byte-p 5 y))
+ :concl (unsigned-byte-p 5 (logand x y)))
+
+(make-event
+ (er-progn (assign :fgl-trace-rewrites nil)
+           (assign :fgl-trace-rule-alist nil)
+           (value '(value-triple :trace-off))))
 
 
-(thm
- (if (and (unsigned-byte-p 5 x)
-          (unsigned-byte-p 5 y))
-     (unsigned-byte-p 5 (logand x y))
-   t)
- :hints (("goal" :clause-processor (gl-interp-cp clause (default-glcp-config) state)
-          :in-theory nil)))
+(fgl-thm
+ :hyp (and (unsigned-byte-p 10 x)
+           (unsigned-byte-p 10 y))
+ :concl (unsigned-byte-p 10 (logand x y)))
 
-(thm
- (if (and (unsigned-byte-p 10 x)
-          (unsigned-byte-p 10 y))
-     (unsigned-byte-p 10 (logand x y))
-   t)
- :hints (("goal" :clause-processor (gl-interp-cp clause (default-glcp-config) state)
-          :in-theory nil)))
+(fgl-thm
+ :hyp (and (unsigned-byte-p 50 x)
+           (unsigned-byte-p 50 y))
+ :concl (unsigned-byte-p 50 (logand x y)))
 
-(thm
- (if (and (unsigned-byte-p 50 x)
-          (unsigned-byte-p 50 y))
-     (unsigned-byte-p 50 (logand x y))
-   t)
- :hints (("goal" :clause-processor (gl-interp-cp clause (default-glcp-config) state)
-          :in-theory nil)))
-
-(thm
- (if (and (unsigned-byte-p 90 x)
-          (unsigned-byte-p 90 y))
-     (unsigned-byte-p 90 (logand x y))
-   t)
- :hints (("goal" :clause-processor (gl-interp-cp clause (default-glcp-config) state)
-          :in-theory nil)))
+(fgl-thm
+  :hyp (and (unsigned-byte-p 90 x)
+            (unsigned-byte-p 90 y))
+  :concl (unsigned-byte-p 90 (logand x y)))
 
 
 ;; (trace$ (gl-rewrite-try-rule
@@ -326,94 +322,94 @@
 
 
 
-(def-gl-rewrite fgl-ash
-  (implies (syntaxp (integerp shift))
-           (equal (ash x shift)
-                  (b* ((x (int x))
-                       (shift (int shift)))
-                    (cond ((eql shift 0) x)
-                          ((< shift 0) (ash (intcdr x) (+ 1 shift)))
-                          (t (intcons nil (ash x (+ -1 shift))))))))
-  :hints(("Goal" :in-theory (enable bitops::ash**
-                                    bitops::logtail**))))
+;; (def-gl-rewrite fgl-ash
+;;   (implies (syntaxp (integerp shift))
+;;            (equal (ash x shift)
+;;                   (b* ((x (int x))
+;;                        (shift (int shift)))
+;;                     (cond ((eql shift 0) x)
+;;                           ((< shift 0) (ash (intcdr x) (+ 1 shift)))
+;;                           (t (intcons nil (ash x (+ -1 shift))))))))
+;;   :hints(("Goal" :in-theory (enable bitops::ash**
+;;                                     bitops::logtail**))))
 
-(define +carry ((c booleanp)
-                (x integerp)
-                (y integerp))
-  (+ (bool->bit c)
-     (lifix x)
-     (lifix y)))
+;; (define +carry ((c booleanp)
+;;                 (x integerp)
+;;                 (y integerp))
+;;   (+ (bool->bit c)
+;;      (lifix x)
+;;      (lifix y)))
 
-(def-gl-rewrite fgl-+carry
-  (equal (+carry c x y)
-         (intcons (xor c (xor (intcar x) (intcar y)))
-                  (if (and (check-int-endp x (syntax-bind xsyn (g-concrete x)))
-                           (check-int-endp y (syntax-bind ysyn (g-concrete y))))
-                      (endint (if c
-                                  (and (intcar x) (intcar y))
-                                (or (intcar x) (intcar y))))
-                    (+carry (if c
-                                (or (intcar x) (intcar y))
-                              (and (intcar x) (intcar y)))
-                            (intcdr x)
-                            (intcdr y)))))
-  :hints(("Goal" :in-theory (enable +carry int-endp
-                                    bitops::equal-logcons-strong
-                                    bitops::logxor** b-not))))
+;; (def-gl-rewrite fgl-+carry
+;;   (equal (+carry c x y)
+;;          (intcons (xor c (xor (intcar x) (intcar y)))
+;;                   (if (and (check-int-endp x (syntax-bind xsyn (g-concrete x)))
+;;                            (check-int-endp y (syntax-bind ysyn (g-concrete y))))
+;;                       (endint (if c
+;;                                   (and (intcar x) (intcar y))
+;;                                 (or (intcar x) (intcar y))))
+;;                     (+carry (if c
+;;                                 (or (intcar x) (intcar y))
+;;                               (and (intcar x) (intcar y)))
+;;                             (intcdr x)
+;;                             (intcdr y)))))
+;;   :hints(("Goal" :in-theory (enable +carry int-endp
+;;                                     bitops::equal-logcons-strong
+;;                                     bitops::logxor** b-not))))
 
-(def-gl-rewrite fgl-+
-  (implies (and (integerp x) (integerp y))
-           (equal (+ x y)
-                  (+carry nil x y)))
-  :hints(("Goal" :in-theory (enable +carry))))
+;; (def-gl-rewrite fgl-+
+;;   (implies (and (integerp x) (integerp y))
+;;            (equal (+ x y)
+;;                   (+carry nil x y)))
+;;   :hints(("Goal" :in-theory (enable +carry))))
 
-(def-gl-rewrite fgl-unary-minus
-  (implies (integerp x)
-           (equal (- x)
-                  (+carry t 0 (lognot x))))
-  :hints(("Goal" :in-theory (enable lognot +carry))))
+;; (def-gl-rewrite fgl-unary-minus
+;;   (implies (integerp x)
+;;            (equal (- x)
+;;                   (+carry t 0 (lognot x))))
+;;   :hints(("Goal" :in-theory (enable lognot +carry))))
 
-(encapsulate nil
-  (local (defthm replace-mult
-           (implies (equal (+ 1 z) x)
-                    (equal (* x y)
-                           (+ y (* z y))))))
-  (local (defthm commute-*-2
-           (equal (* y x z) (* x y z))
-           :hints (("goal" :use ((:instance associativity-of-*)
-                                 (:instance associativity-of-*
-                                  (x y) (y x)))
-                    :in-theory (disable associativity-of-*)))))
+;; (encapsulate nil
+;;   (local (defthm replace-mult
+;;            (implies (equal (+ 1 z) x)
+;;                     (equal (* x y)
+;;                            (+ y (* z y))))))
+;;   (local (defthm commute-*-2
+;;            (equal (* y x z) (* x y z))
+;;            :hints (("goal" :use ((:instance associativity-of-*)
+;;                                  (:instance associativity-of-*
+;;                                   (x y) (y x)))
+;;                     :in-theory (disable associativity-of-*)))))
 
-  (def-gl-rewrite fgl-*
-    (implies (and (integerp x) (integerp y))
-             (equal (* x y)
-                    (if (check-int-endp x (syntax-bind xsyn (g-concrete x)))
-                        (if (intcar x) (- y) 0)
-                      (+ (if (intcar x) y 0)
-                         (intcons nil
-                                  (* (intcdr x) y))))))
-    :hints(("Goal" :in-theory (e/d (int-endp logcons)
-                                   (acl2::logcar-logcdr-elim
-                                    bitops::logcons-destruct))
-            :use ((:instance acl2::logcar-logcdr-elim
-                   (i x)))))))
+;;   (def-gl-rewrite fgl-*
+;;     (implies (and (integerp x) (integerp y))
+;;              (equal (* x y)
+;;                     (if (check-int-endp x (syntax-bind xsyn (g-concrete x)))
+;;                         (if (intcar x) (- y) 0)
+;;                       (+ (if (intcar x) y 0)
+;;                          (intcons nil
+;;                                   (* (intcdr x) y))))))
+;;     :hints(("Goal" :in-theory (e/d (int-endp logcons)
+;;                                    (acl2::logcar-logcdr-elim
+;;                                     bitops::logcons-destruct))
+;;             :use ((:instance acl2::logcar-logcdr-elim
+;;                    (i x)))))))
 
-(def-gl-rewrite fgl-lognot
-  (equal (lognot x)
-         (if (check-int-endp x (syntax-bind xsyn (g-concrete x)))
-             (endint (not (intcar x)))
-           (intcons (not (intcar x))
-                    (lognot (intcdr x)))))
-  :hints(("Goal" :in-theory (enable bitops::lognot** int-endp))))
+;; (def-gl-rewrite fgl-lognot
+;;   (equal (lognot x)
+;;          (if (check-int-endp x (syntax-bind xsyn (g-concrete x)))
+;;              (endint (not (intcar x)))
+;;            (intcons (not (intcar x))
+;;                     (lognot (intcdr x)))))
+;;   :hints(("Goal" :in-theory (enable bitops::lognot** int-endp))))
 
-(def-gl-rewrite fgl-negp
-  (implies (integerp x)
-           (equal (acl2::negp x)
-                  (if (check-int-endp x (syntax-bind xsyn (g-concrete x)))
-                      (intcar x)
-                    (acl2::negp (intcdr x)))))
-  :hints(("Goal" :in-theory (enable int-endp))))
+;; (def-gl-rewrite fgl-negp
+;;   (implies (integerp x)
+;;            (equal (acl2::negp x)
+;;                   (if (check-int-endp x (syntax-bind xsyn (g-concrete x)))
+;;                       (intcar x)
+;;                     (acl2::negp (intcdr x)))))
+;;   :hints(("Goal" :in-theory (enable int-endp))))
 
 ;; (define count-nat-bits ((x natp))
 ;;   :measure (integer-length x)
@@ -449,23 +445,30 @@
 ;;                 (count-int-bits val (intcdr x)))))
 ;;     :hints(("Goal" :in-theory (enable int-endp)))))
 
-(def-gl-rewrite fgl-logcount
-  (equal (logcount x)
-         (b* ((x (int x)))
-           (if (check-int-endp x (syntax-bind xsyn (g-concrete x)))
-               0
-             (if (acl2::negp x)
-                 (if (eql x -1)
-                     0
-                   (+ (bool->bit (not (intcar x)))
-                      (logcount (intcdr x))))
-               (if (eql x 0)
-                   0
-                 (+ (bool->bit (intcar x))
-                    (logcount (intcdr x))))))))
-  :hints(("Goal" :in-theory (enable int-endp
-                                    bitops::logcount**))))
-                  
+;; (def-gl-rewrite fgl-logcount
+;;   (equal (logcount x)
+;;          (b* ((x (int x)))
+;;            (if (check-int-endp x (syntax-bind xsyn (g-concrete x)))
+;;                0
+;;              (if (acl2::negp x)
+;;                  (if (eql x -1)
+;;                      0
+;;                    (+ (bool->bit (not (intcar x)))
+;;                       (logcount (intcdr x))))
+;;                (if (eql x 0)
+;;                    0
+;;                  (+ (bool->bit (intcar x))
+;;                     (logcount (intcdr x))))))))
+;;   :hints(("Goal" :in-theory (enable int-endp
+;;                                     bitops::logcount**))))
+
+(make-event
+ (er-progn (assign :fgl-trace-rule-alist '(((:rewrite fgl-*))
+                                           ((:rewrite <-impl))
+                                           ((:rewrite fgl-logcount))
+                                           ((:rewrite logcount-impl))
+                                           ((:rewrite +-to-+carry-width))))
+           (value '(value-triple :trace-rules))))
 
 (defun 32* (x y)
   (logand (* x y) (1- (expt 2 32))))
@@ -479,13 +482,10 @@
               #x1010101)
          -24)))
 
-(thm
- (if (unsigned-byte-p 32 x)
-     (equal (fast-logcount-32 x)
-            (logcount x))
-   t)
- :hints (("goal" :clause-processor (gl-interp-cp clause (default-glcp-config) state)
-          :in-theory nil)))
+(fgl-thm
+ :hyp (unsigned-byte-p 32 x)
+ :concl (equal (fast-logcount-32 x)
+               (logcount x)))
 
 
   
@@ -500,50 +500,39 @@
               #x1010101)
          -24)))
 
+(make-event
+ (b* (((mv err ?val state)
+       (fgl-thm
+        :hyp (unsigned-byte-p 32 x)
+        :concl (equal (fast-logcount-32* x)
+                      (logcount x))))
+      ((unless err)
+       (er soft 'ctrex-test "Expected this to fail!~%"))
+      (x-look (assoc-equal 'x (@ fgl-interp-error-debug-obj)))
+      ((unless x-look)
+       (er soft 'ctrex-test "Expected a counterexample binding for X~%"))
+      (x (cdr x-look))
+      ((unless (and (unsigned-byte-p 32 x)
+                    (not (equal (fast-logcount-32* x)
+                                (logcount x)))))
+       (er soft 'ctrex-test "Bad counterexample!~%")))
+   (value '(value-triple :ok))))
 
 
 
-(defun show-counterexample ()
-  nil)
-
-(table gl-fn-modes 'show-counterexample
-       (make-gl-function-mode :dont-concrete-exec t))
-
-(def-gl-rewrite show-counterexample-rw
-  (equal (show-counterexample)
-         (b* (((list bindings vars)
-               (syntax-bind alists
-                            (mv-let (bindings-vals var-vals)
-                              (interp-st-counterex-stack-prev-bindings/print-errors interp-st state)
-                              (g-concrete (list bindings-vals var-vals))))))
-           (cw "Counterexample -- bindings: ~x0 variables: ~x1~%"
-               bindings vars))))
-              
-                                   
 
 (make-event
- ;; The must-fail doesn't really do it
- '(:or (thm
+ (b* (((mv err ?val state)
+       (fgl-thm
+        :hyp t
+        :concl
         ;; (if (unsigned-byte-p 32 x)
         (b* ((x (loghead 32 xx))
              (impl (fast-logcount-32* x))
              (spec (logcount x))
              (eq (equal impl spec))
-             (?uneq-sat (fgl-sat-check (make-fgl-sat-config) (not eq))))
-          (show-counterexample))
-        ;;    (alists (syntax-bind alists1
-        ;;                         (mv-let (bindings-vals var-vals)
-        ;;                           (interp-st-counterex-stack-bindings/print-errors interp-st state)
-        ;;                           (g-concrete (list bindings-vals var-vals))))))
-        ;; (cw "Counterexample!: alists: ~x0~%" alists))
-        :hints (("goal" :clause-processor (gl-interp-cp clause (default-glcp-config) state)
-                 :in-theory nil)))
-   (value-triple :failed-as-expected)))
-
-
-;; (thm
-;;  (implies (unsigned-byte-p 32 x)
-;;           (equal (fast-logcount-32 x)
-;;                  (logcount x)))
-;;  :hints (("goal" :clause-processor (gl-interp-cp clause (default-glcp-config) state)
-;;           :in-theory nil)))
+             (?uneq-sat (fgl-sat-check (make-fgl-ipasir-config) (not eq))))
+          (show-counterexample "unequal"))))
+      ((unless err)
+       (er soft 'ctrex-test "Expected this to fail!~%")))
+   (value '(value-triple :ok))))
