books/centaur/fgl/trace.lisp
@@ -1,0 +1,133 @@
+; GL - A Symbolic Simulation Framework for ACL2
+; Copyright (C) 2019 Centaur Technology
+;
+; Contact:
+;   Centaur Technology Formal Verification Group
+;   7600-C N. Capital of Texas Highway, Suite 300, Austin, TX 78731, USA.
+;   http://www.centtech.com/
+;
+; License: (An MIT/X11-style license)
+;
+;   Permission is hereby granted, free of charge, to any person obtaining a
+;   copy of this software and associated documentation files (the "Software"),
+;   to deal in the Software without restriction, including without limitation
+;   the rights to use, copy, modify, merge, publish, distribute, sublicense,
+;   and/or sell copies of the Software, and to permit persons to whom the
+;   Software is furnished to do so, subject to the following conditions:
+;
+;   The above copyright notice and this permission notice shall be included in
+;   all copies or substantial portions of the Software.
+;
+;   THE SOFTWARE IS PROVIDED "AS IS", WITHOUT WARRANTY OF ANY KIND, EXPRESS OR
+;   IMPLIED, INCLUDING BUT NOT LIMITED TO THE WARRANTIES OF MERCHANTABILITY,
+;   FITNESS FOR A PARTICULAR PURPOSE AND NONINFRINGEMENT. IN NO EVENT SHALL THE
+;   AUTHORS OR COPYRIGHT HOLDERS BE LIABLE FOR ANY CLAIM, DAMAGES OR OTHER
+;   LIABILITY, WHETHER IN AN ACTION OF CONTRACT, TORT OR OTHERWISE, ARISING
+;   FROM, OUT OF OR IN CONNECTION WITH THE SOFTWARE OR THE USE OR OTHER
+;   DEALINGS IN THE SOFTWARE.
+;
+; Original author: Sol Swords <sswords@centtech.com>
+
+(in-package "FGL")
+
+(include-book "interp-st")
+
+
+
+
+(encapsulate
+  (((gl-rewrite-try-rule-trace * * * * interp-st state) => interp-st
+    :formals (status rule fn args interp-st state)
+    :guard t))
+
+  (set-ignore-ok t)
+  (set-irrelevant-formals-ok t)
+  (local (defun gl-rewrite-try-rule-trace (status rule fn args interp-st state)
+           (declare (xargs :stobjs (interp-st state)))
+           interp-st))
+
+  (defthm interp-st-get-of-gl-rewrite-try-rule-trace
+    (implies (not (equal (interp-st-field-fix key) :trace-scratch))
+             (equal (interp-st-get key (gl-rewrite-try-rule-trace status rule fn args interp-st state))
+                    (interp-st-get key interp-st)))))
+
+(define gl-rewrite-try-rule-trace-wrapper (trace status rule fn args interp-st state)
+  :inline t
+  (if trace
+      (gl-rewrite-try-rule-trace status rule fn args interp-st state)
+    interp-st)
+  ///
+  (defthm interp-st-get-of-gl-rewrite-try-rule-trace-wrapper
+    (implies (not (equal (interp-st-field-fix key) :trace-scratch))
+             (equal (interp-st-get key (gl-rewrite-try-rule-trace-wrapper
+                                        trace status rule fn args interp-st state))
+                    (interp-st-get key interp-st)))))
+
+
+(define gl-rewrite-rule-try-trace-default (status rule fn args interp-st state)
+  :returns new-interp-st
+  (b* ((rule-alist (and (boundp-global :fgl-trace-rule-alist state)
+                        (@ :fgl-trace-rule-alist)))
+       ((unless (and (consp rule)
+                     (consp (cdr rule))
+                     (alistp rule-alist)))
+        ;; needed to access the rune
+        (prog2$ (cw "bad rule~%")
+                interp-st))
+       (rune (cadr rule))
+       (look (assoc-equal rune rule-alist))
+       ((unless look)
+        interp-st)
+       (depth (nfix (interp-st->trace-scratch interp-st)))
+       (evisc-tuple (and (boundp-global :fgl-trace-evisc-tuple state)
+                         (@ :fgl-trace-evisc-tuple))))
+    (case-match status
+      (':start
+       (prog2$ (fmt-to-comment-window
+                "~t0~x1> ~x2 ~x3~%"
+                (pairlis2 acl2::*base-10-chars* (list depth depth rune (cons fn args)))
+                0 evisc-tuple nil)
+               (update-interp-st->trace-scratch (1+ depth) interp-st)))
+      ((':hyps . failed-hyp)
+       (b* ((errmsg (interp-st->errmsg interp-st))
+            ((when errmsg)
+             (fmt-to-comment-window
+              "~t0<~x1 ~x2 failed (error in hyps: ~@3)~%"
+              (pairlis2 acl2::*base-10-chars* (list (1- depth) (1- depth) rune
+                                                    (if (msgp errmsg)
+                                                        errmsg
+                                                      (msg "~x0" errmsg))))
+              0 evisc-tuple nil)
+             (update-interp-st->trace-scratch (1- depth) interp-st))
+            ((when failed-hyp)
+             (fmt-to-comment-window
+              "~t0<~x1 ~x2 failed (hyp ~x3)~%"
+              (pairlis2 acl2::*base-10-chars* (list (1- depth) depth rune failed-hyp))
+              0 evisc-tuple nil)
+             (update-interp-st->trace-scratch (1- depth) interp-st)))
+         interp-st))
+      ((':finish . val)
+       (b* ((errmsg (interp-st->errmsg interp-st))
+            ((when errmsg)
+             (fmt-to-comment-window
+              "~t0<~x1 ~x2 failed (error: ~@3)~%"
+              (pairlis2 acl2::*base-10-chars* (list (1- depth) (1- depth) rune
+                                                    (if (msgp errmsg)
+                                                        errmsg
+                                                      (msg "~x0" errmsg))))
+              0 evisc-tuple nil)
+             (update-interp-st->trace-scratch (1- depth) interp-st)))
+         (fmt-to-comment-window
+          "~t0<~x1 ~x2 success: ~x3~%"
+          (pairlis2 acl2::*base-10-chars* (list (1- depth) (1- depth) rune val))
+          0 evisc-tuple nil)
+         (update-interp-st->trace-scratch (1- depth) interp-st)))
+      (& (prog2$ (cw "bad status: ~x0~%" status)
+                 interp-st))))
+  ///
+  (defret interp-st-get-of-<fn>
+    (implies (not (Equal (interp-st-field-fix key) :trace-scratch))
+             (equal (interp-st-get key new-interp-st)
+                    (interp-st-get key interp-st)))))
+
+(defattach gl-rewrite-try-rule-trace gl-rewrite-rule-try-trace-default)
